LeanSAT/Reflect/BVExpr/BitBlastLemmas.lean
@@ -1,0 +1,180 @@
+import LeanSAT.Reflect.BVExpr.BitBlast
+
+open AIG
+
+namespace BVExpr
+
+def Assignment.toAIGAssignment (assign : Assignment) : BVBit → Bool :=
+  fun bit => (assign.getD bit.var).bv.getLsb bit.idx
+
+@[simp]
+theorem Assignment.toAIGAssignment_apply (assign : Assignment) (bit : BVBit)
+    : assign.toAIGAssignment bit = (assign.getD bit.var).bv.getLsb bit.idx := by
+  rfl
+
+theorem bitblast.go_val_eq_bitblast (aig : AIG BVBit) (expr : BVExpr w) (idx : Nat) (hidx : idx < w)
+    : (go aig expr idx hidx).val = bitblast aig ⟨expr, idx, hidx⟩ := by
+  rfl
+
+theorem bitblast.go_denote_eq_eval (aig : AIG BVBit) (expr : BVExpr w) (idx : Nat) (hidx : idx < w)
+    (assign : Assignment)
+    : ⟦(bitblast.go aig expr idx hidx).val, assign.toAIGAssignment⟧
+        =
+      (expr.eval assign).getLsb idx := by
+  induction expr generalizing aig with
+  | var =>
+    simp [go, hidx]
+  | const =>
+    simp [go]
+  | bin lhs op rhs lih rih =>
+    cases op with
+    | and =>
+      simp only [go, denote_mkAndCached, Ref_cast, Ref_ofEntrypoint, rih, eval_bin,
+        BVBinOp.eval_and, BitVec.getLsb_and]
+      simp only [bitblast.go_val_eq_bitblast (go aig lhs idx hidx).val.aig]
+      rw [LawfulOperator.denote_input_entry (f := bitblast)]
+      rw [lih]
+  | un op expr ih =>
+    cases op with
+    | not =>
+      simp [go, ih, hidx]
+
+@[simp]
+theorem bitblast_denote_eq_eval_getLsb (aig : AIG BVBit) (target : SingleBit) (assign : Assignment)
+    : ⟦bitblast aig target, assign.toAIGAssignment⟧
+        =
+      (target.expr.eval assign).getLsb target.idx := by
+  unfold bitblast
+  rw [bitblast.go_denote_eq_eval]
+
+@[simp]
+theorem mkBitEq_denote_eq_eval_getLsb_eq (aig : AIG BVBit) (pair : BitPair) (assign : Assignment)
+    : ⟦mkBitEq aig pair, assign.toAIGAssignment⟧
+        =
+      (
+        (pair.lhs.eval assign).getLsb pair.idx
+          ==
+        (pair.rhs.eval assign).getLsb pair.idx
+      ) := by
+  unfold mkBitEq
+  -- TODO: potentially more theory around BitPair
+  simp [LawfulOperator.denote_input_entry (f := bitblast), BitPair.leftBit, BitPair.rightBit]
+
+end BVExpr
+
+namespace BVPred
+
+theorem mkEq.go_denote_eq_eval (aig : AIG BVBit) (lhs rhs : BVExpr w) (idx : Nat) (hidx : idx ≤ w)
+    (assign : BVExpr.Assignment)
+    : ⟦go aig lhs rhs idx hidx, assign.toAIGAssignment⟧
+        ↔
+      (∀ bit < idx, (lhs.eval assign).getLsb bit = (rhs.eval assign).getLsb bit) := by
+  induction idx using Nat.caseStrongInductionOn with
+  | zero =>
+    simp only [go, mkConstCached_eval_eq_mkConst_eval, denote_mkConst, Nat.zero_eq, true_iff]
+    intro bit hbit
+    contradiction
+  | ind idx ih =>
+    constructor
+    . intro h bit hbit
+      specialize ih idx (by omega) (by omega)
+      simp only [go, denote_mkAndCached, Ref_ofEntrypoint, denote_projected_entry,
+        BVExpr.mkBitEq_denote_eq_eval_getLsb_eq, Ref_cast, Bool.and_eq_true, beq_iff_eq] at h
+      rcases h with ⟨hl, hr⟩
+      rw [LawfulOperator.denote_input_entry (f := BVExpr.mkBitEq)] at hr
+      simp only [hr, true_iff] at ih
+      have : bit ≤ idx := by omega
+      cases Nat.eq_or_lt_of_le this with
+      | inl h =>
+        rw [h]
+        assumption
+      | inr h =>
+        apply ih
+        assumption
+    . intro h
+      simp only [go, denote_mkAndCached, Ref_ofEntrypoint, denote_projected_entry,
+        BVExpr.mkBitEq_denote_eq_eval_getLsb_eq, Ref_cast, Bool.and_eq_true, beq_iff_eq]
+      constructor
+      . apply h
+        omega
+      . rw [LawfulOperator.denote_input_entry (f := BVExpr.mkBitEq)]
+        rw [ih]
+        . intro bit hbit
+          apply h
+          omega
+        . omega
+
+theorem mkEq_denote_iff_eval_beq (aig : AIG BVBit) (pair : ExprPair) (assign : BVExpr.Assignment)
+    : ⟦mkEq aig pair, assign.toAIGAssignment⟧
+        ↔
+      (pair.lhs.eval assign == pair.rhs.eval assign) := by
+  rw [beq_iff_eq]
+  unfold mkEq
+  rw [mkEq.go_denote_eq_eval]
+  constructor
+  . intro h
+    apply BitVec.eq_of_getLsb_eq
+    intro i
+    specialize h i.val i.isLt
+    assumption
+  . intro h _ _
+    rw [h]
+
+
+@[simp]
+theorem mkEq_denote_eq_eval_beq (aig : AIG BVBit) (pair : ExprPair) (assign : BVExpr.Assignment)
+    : ⟦mkEq aig pair, assign.toAIGAssignment⟧
+        =
+      (pair.lhs.eval assign == pair.rhs.eval assign) := by
+  rw [Bool.eq_iff_iff]
+  apply mkEq_denote_iff_eval_beq
+
+theorem mkNeq_denote_iff_eval_neq (aig : AIG BVBit) (pair : ExprPair) (assign : BVExpr.Assignment)
+    : ⟦mkNeq aig pair, assign.toAIGAssignment⟧
+        ↔
+      (pair.lhs.eval assign != pair.rhs.eval assign) := by
+  unfold mkNeq
+  simp
+
+@[simp]
+theorem mkNeq_denote_eq_eval_neq (aig : AIG BVBit) (pair : ExprPair) (assign : BVExpr.Assignment)
+    : ⟦mkNeq aig pair, assign.toAIGAssignment⟧
+        =
+      (pair.lhs.eval assign != pair.rhs.eval assign) := by
+  rw [Bool.eq_iff_iff]
+  apply mkNeq_denote_iff_eval_neq
+
+@[simp]
+theorem bitblast_denote_eq_eval (aig : AIG BVBit) (pred : BVPred) (assign : BVExpr.Assignment)
+    : ⟦bitblast aig pred, assign.toAIGAssignment⟧
+        =
+      pred.eval assign := by
+  cases pred with
+  | bin lhs op rhs =>
+    cases op with
+    | eq => simp [bitblast]
+    | neq => simp [bitblast]
+
+end BVPred
+
+namespace BVLogicalExpr
+
+theorem bitblast.go_eval_eq_eval (expr : BVLogicalExpr) (aig : AIG BVBit) (assign : BVExpr.Assignment) :
+    ⟦ofBoolExprCached.go BVPred.bitblast expr aig, assign.toAIGAssignment⟧ = expr.eval assign := by
+  induction expr generalizing aig with
+  | const => simp [ofBoolExprCached.go]
+  | literal => simp [ofBoolExprCached.go]
+  | not expr ih => simp [ofBoolExprCached.go, ih]
+  | gate g lhs rhs lih rih => cases g <;> simp [ofBoolExprCached.go, Gate.eval, lih, rih]
+
+@[simp]
+theorem bitblast_denote_eq_eval (expr : BVLogicalExpr) (assign : BVExpr.Assignment)
+    : ⟦bitblast expr, assign.toAIGAssignment⟧
+        =
+      expr.eval assign := by
+  unfold bitblast
+  unfold ofBoolExprCached
+  rw [bitblast.go_eval_eq_eval]
+
+
+end BVLogicalExpr
